C-verifier/src/Midend-IVL/Isabelle-UTP-Extended/theories/Rel/utp_rel_more.thy
@@ -1,0 +1,132 @@
+(******************************************************************************
+ * Orca: A Functional Correctness Verifier for Imperative Programs
+ *       Based on Isabelle/UTP
+ *
+ * Copyright (c) 2016-2018 Virginia Tech, USA
+ *               2016-2018 Technische Universität München, Germany
+ *               2016-2018 University of York, UK
+ *               2016-2018 Université Paris-Saclay, Univ. Paris-Sud, France
+ *
+ * This software may be distributed and modified according to the terms of
+ * the GNU Lesser General Public License version 3.0 or any later version.
+ * Note that NO WARRANTY is provided.
+ *
+ * See CONTRIBUTORS, LICENSE and CITATION files for details.
+ ******************************************************************************)
+
+theory utp_rel_more
+imports   "../../../Isabelle-UTP/utp/utp_rel"
+begin
+section \<open>More on Rel programs\<close> 
+subsection \<open>SKIP\<close>  
+  
+abbreviation skip'::"'\<alpha> hrel" ("SKIP")
+  where "SKIP \<equiv> skip_r" 
+    
+subsection \<open>conditional\<close>  
+
+abbreviation rcond'::"'\<alpha> cond \<Rightarrow> '\<alpha> hrel \<Rightarrow>  '\<alpha> hrel \<Rightarrow> '\<alpha> hrel" ("bif (_)/ then (_) else (_) eif")
+where "bif b then P else Q eif \<equiv> (P \<triangleleft> \<lceil>b\<rceil>\<^sub>< \<triangleright> Q)"  
+
+subsection \<open>Iterations and loops \<close>
+text \<open>We propose a generic scheme fro iterations inspired by eiffel~\url{https://www.ecma-international.org/publications/files/ECMA-ST/ECMA-367.pdf}.
+      The same scheme was used in~url{https://arxiv.org/pdf/1211.4470.pdf}. 
+      Since this iteration scheme is generic all other iterations can be derived from it.\<close>
+  
+definition from_until_gfp_rel :: "'\<alpha> hrel \<Rightarrow>'\<alpha> cond \<Rightarrow> '\<alpha> hrel \<Rightarrow> '\<alpha> hrel" ("from\<^sup>\<top> _ until _ do _ od") 
+  where "from\<^sup>\<top> init until exit do body od =  
+         init ;; (\<nu> X \<bullet> bif \<not> exit then (body ;; X) else SKIP eif)" 
+  
+definition from_until_lfp_rel :: "'\<alpha> hrel \<Rightarrow>'\<alpha> cond \<Rightarrow> '\<alpha> hrel \<Rightarrow> '\<alpha> hrel" ("from\<^sub>\<bottom> _ until _ do _ od") 
+  where "from\<^sub>\<bottom> init until exit do body od =  
+         init ;; (\<mu> X \<bullet> bif \<not> exit then (body ;; X) else SKIP eif)" 
+
+definition while_gfp_rel :: "'\<alpha> cond \<Rightarrow> '\<alpha> hrel \<Rightarrow> '\<alpha> hrel" ("while\<^sup>\<top> _ do _ od")
+where "while\<^sup>\<top> b do body od = from\<^sup>\<top> SKIP until \<not> b do body od"
+
+definition while_lfp_rel :: "'\<alpha> cond \<Rightarrow> '\<alpha> hrel \<Rightarrow> '\<alpha> hrel" ("while\<^sub>\<bottom> _ do _ od") 
+  where "while\<^sub>\<bottom> b do body od =  from\<^sub>\<bottom> SKIP until \<not> b do body od"
+    
+definition do_while_gfp_rel :: 
+  "'\<alpha> hrel \<Rightarrow> '\<alpha> cond \<Rightarrow> '\<alpha> hrel" ("do _ while\<^sup>\<top> _ od")
+where "do body while\<^sup>\<top> b od = from\<^sup>\<top> body until \<not> b do body od"
+
+definition do_while_lfp_rel :: 
+  "'\<alpha> hrel \<Rightarrow> '\<alpha> cond \<Rightarrow>  '\<alpha> hrel" ("do _ while\<^sub>\<bottom> _ od") 
+  where "do body while\<^sub>\<bottom> b od = from\<^sub>\<bottom> body until \<not> b do body od"
+    
+definition for_gfp_rel :: 
+  "'\<alpha> hrel \<Rightarrow> '\<alpha> cond \<Rightarrow> '\<alpha> hrel \<Rightarrow> '\<alpha> hrel \<Rightarrow> '\<alpha> hrel" ("for\<^sup>\<top> '(_,_,_') do _ od")
+where "for\<^sup>\<top> (init, b, incr) do body od = from\<^sup>\<top> init until \<not> b do body ;; incr od"
+
+definition for_lfp_rel:: 
+  "'\<alpha> hrel \<Rightarrow> '\<alpha> cond \<Rightarrow> '\<alpha> hrel \<Rightarrow> '\<alpha> hrel \<Rightarrow> '\<alpha> hrel" ("for\<^sub>\<bottom> '(_,_,_') do _ od")
+where "for\<^sub>\<bottom> (init, b, incr) do body od = from\<^sub>\<bottom> init until \<not> b do body ;; incr od"
+    
+text \<open>Iterations with invariant decoration\<close>
+
+definition from_until_lfp_invr_rel :: "'\<alpha> hrel \<Rightarrow> '\<alpha> cond \<Rightarrow> '\<alpha> cond \<Rightarrow> '\<alpha> hrel \<Rightarrow> '\<alpha> hrel" ("from\<^sub>\<bottom> _ invr _ until _ do _ od") 
+  where "from\<^sub>\<bottom> init invr invar  until exit do body od = from\<^sub>\<bottom> init until exit do body od"
+
+definition from_until_gfp_invr_rel :: "'\<alpha> hrel \<Rightarrow> '\<alpha> cond \<Rightarrow> '\<alpha> cond \<Rightarrow> '\<alpha> hrel \<Rightarrow> '\<alpha> hrel" ("from\<^sup>\<top> _ invr _ until _ do _ od") 
+  where "from\<^sup>\<top> init invr invar until exit do body od = from\<^sup>\<top> init until exit do body od"
+
+definition while_lfp_invr_rel :: "'\<alpha> cond \<Rightarrow> '\<alpha> cond \<Rightarrow> '\<alpha> hrel \<Rightarrow> '\<alpha> hrel" ("invr _ while\<^sub>\<bottom> _ do _ od") 
+where "invr invar while\<^sub>\<bottom> b do body od = while\<^sub>\<bottom> b do body od"
+
+definition while_gfp_invr_rel :: "'\<alpha> cond \<Rightarrow> '\<alpha> cond \<Rightarrow> '\<alpha> hrel \<Rightarrow> '\<alpha> hrel" ("invr _ while\<^sup>\<top> _ do _ od") 
+where "invr invar while\<^sup>\<top> b do body od = while\<^sup>\<top> b do body od"
+
+definition do_while_gfp_invr_rel :: 
+  "'\<alpha> hrel \<Rightarrow> '\<alpha> cond \<Rightarrow> '\<alpha> cond \<Rightarrow> '\<alpha> hrel" ("do _ while\<^sup>\<top> _ invr _ od")
+where "do body while\<^sup>\<top> b invr invar od = from\<^sup>\<top> body until \<not> b do body od"
+
+definition do_while_lfp_invr_rel :: 
+  "'\<alpha> hrel \<Rightarrow> '\<alpha> cond \<Rightarrow> '\<alpha> cond \<Rightarrow> '\<alpha> hrel" ("do _ while\<^sub>\<bottom> _ invr _ od") 
+where "do body while\<^sub>\<bottom> b invr invar od = from\<^sub>\<bottom> body until \<not> b do body od"  
+  
+definition for_gfp_invr_rel :: 
+  "'\<alpha> hrel \<Rightarrow> '\<alpha> cond \<Rightarrow> '\<alpha> hrel \<Rightarrow> '\<alpha> cond \<Rightarrow> '\<alpha> hrel \<Rightarrow> '\<alpha> hrel" ("for\<^sup>\<top> '(_,_,_') invr _ do _ od")
+where "for\<^sup>\<top> (init, b, incr) invr invar do body od = from\<^sup>\<top> init until \<not> b do body ;; incr od"
+
+definition for_lfp_invr_rel :: 
+  "'\<alpha> hrel \<Rightarrow> '\<alpha> cond \<Rightarrow> '\<alpha> hrel \<Rightarrow> '\<alpha> cond \<Rightarrow>  '\<alpha> hrel \<Rightarrow> '\<alpha> hrel" ("for\<^sub>\<bottom> '(_,_,_') invr _ do _ od")
+where "for\<^sub>\<bottom> (init, b, incr) invr invar do body od = from\<^sub>\<bottom> init until \<not> b do body ;; incr od"
+  
+text \<open>Iterations with invariant and variant decoration\<close>
+  
+definition from_until_lfp_invr_vrt_rel :: 
+  "'\<alpha> hrel \<Rightarrow>'\<alpha> cond \<Rightarrow> ('t,'\<alpha>) uexpr \<Rightarrow> '\<alpha> cond \<Rightarrow> '\<alpha> hrel \<Rightarrow> '\<alpha> hrel" ("from\<^sub>\<bottom> _ invr _ vrt _ until _ do _ od") 
+  where "from\<^sub>\<bottom> init invr invar vrt vari until exit do body od =  from\<^sub>\<bottom> init until exit do body od"
+
+definition from_until_gfp_invr_vrt_rel :: 
+  "'\<alpha> hrel \<Rightarrow>'\<alpha> cond \<Rightarrow> ('t,'\<alpha>) uexpr \<Rightarrow> '\<alpha> cond \<Rightarrow> '\<alpha> hrel \<Rightarrow> '\<alpha> hrel" ("from\<^sup>\<top> _ invr _ vrt _ until _ do _ od") 
+  where "from\<^sup>\<top> init invr invar vrt vari until exit do body od =  from\<^sup>\<top> init until exit do body od"
+    
+definition while_lfp_invr_vrt_rel :: 
+  "'\<alpha> cond \<Rightarrow> ('t,'\<alpha>) uexpr \<Rightarrow>  '\<alpha> cond \<Rightarrow> '\<alpha> hrel \<Rightarrow> '\<alpha> hrel" ("invr _ vrt _ while\<^sub>\<bottom> _ do _ od") 
+where "invr invar vrt vari while\<^sub>\<bottom> b do body od = while\<^sub>\<bottom> b do body od"
+
+definition while_gfp_invr_vrt_rel :: 
+  "'\<alpha> cond \<Rightarrow> ('t,'\<alpha>) uexpr \<Rightarrow>  '\<alpha> cond \<Rightarrow> '\<alpha> hrel \<Rightarrow> '\<alpha> hrel" ("invr _ vrt _ while\<^sup>\<top> _ do _ od") 
+where "invr invar vrt vari while\<^sup>\<top> b do body od = while\<^sup>\<top> b do body od"
+
+definition do_while_gfp_invr_vrt_rel :: 
+   "'\<alpha> hrel \<Rightarrow> '\<alpha> cond \<Rightarrow> '\<alpha> cond \<Rightarrow> ('t,'\<alpha>) uexpr \<Rightarrow> '\<alpha> hrel" ("do _ while\<^sup>\<top> _ invr _ vrt _ od")
+where "do body while\<^sup>\<top> b invr invar vrt vari od = from\<^sup>\<top> body until \<not> b do body od"
+
+definition do_while_lfp_invr_vrt_rel :: 
+   "'\<alpha> hrel \<Rightarrow> '\<alpha> cond \<Rightarrow> '\<alpha> cond \<Rightarrow> ('t,'\<alpha>) uexpr \<Rightarrow> '\<alpha> hrel" ("do _ while\<^sub>\<bottom> _ invr _ vrt _ od") 
+   where "do body while\<^sub>\<bottom> b invr invar vrt vari od = from\<^sub>\<bottom> body until \<not> b do body od"
+     
+definition for_gfp_invr_vrt_rel :: 
+  "'\<alpha> hrel \<Rightarrow> '\<alpha> cond \<Rightarrow> '\<alpha> hrel \<Rightarrow> '\<alpha> cond \<Rightarrow> ('t,'\<alpha>) uexpr \<Rightarrow> '\<alpha> hrel \<Rightarrow> '\<alpha> hrel" ("for\<^sup>\<top> '(_,_,_') invr _ vrt_ do _ od")
+where "for\<^sup>\<top> (init, b, incr) invr invar vrt vari do body od = from\<^sup>\<top> init until \<not> b do body ;; incr od"
+
+definition for_lfp_invr_vrt_rel :: 
+  "'\<alpha> hrel \<Rightarrow> '\<alpha> cond \<Rightarrow> '\<alpha> hrel \<Rightarrow> '\<alpha> cond \<Rightarrow> ('t,'\<alpha>) uexpr \<Rightarrow> '\<alpha> hrel \<Rightarrow> '\<alpha> hrel" ("for\<^sub>\<bottom> '(_,_,_') invr _ vrt _ do _ od")
+where "for\<^sub>\<bottom> (init, b, incr) invr invar vrt vari do body od = from\<^sub>\<bottom> init until \<not> b do body ;; incr od"
+ 
+
+end
+
